Ctyping: better typing of conditional expressions. Ctyping: define a typechecker for whole programs. Csyntax: introduce the type "pre-program" (non-dependent). C2C: use Ctyping.econdition instead of Ctyping.econdition'.
Note: Ctyping.typecheck_program could be used as the first step
in the verified compilation pipeline.  Then, retyping would
no longer be performed in C2C.  We keep it this way (for the time
being) because retyping errors are reported more precisely in C2C than
in Ctyping.

cfrontend/C2C.ml
@@ -626,7 +626,6 @@ let ewrap = function
       error ("retyping error: " ^  string_of_errmsg msg); ezero
 
 let rec convertExpr env e =
-  (*let ty = convertTyp env e.etyp in*)
   match e.edesc with
   | C.EVar _
   | C.EUnop((C.Oderef|C.Odot _|C.Oarrow _), _)
@@ -734,9 +733,8 @@ let rec convertExpr env e =
       ewrap (Ctyping.eseqor (convertExpr env e1) (convertExpr env e2))
 
   | C.EConditional(e1, e2, e3) ->
-      ewrap (Ctyping.econdition' (convertExpr env e1)
-                                     (convertExpr env e2) (convertExpr env e3)
-                                     (convertTyp env e.etyp))
+      ewrap (Ctyping.econdition (convertExpr env e1)
+                                (convertExpr env e2) (convertExpr env e3))
   | C.ECast(ty1, e1) ->
       ewrap (Ctyping.ecast (convertTyp env ty1) (convertExpr env e1))
   | C.ECompound(ty1, ie) ->
